Checkpoint

Core.v
@@ -1,32 +1,76 @@
-From Stdlib Require Import Arith.
+Require Import ExtLib.Structures.Functor.
+Require Import ExtLib.Structures.Monad.
+Import MonadNotation.
+Open Scope monad_scope.
+Require Import ExtLib.Data.Monads.OptionMonad.
 
 Set Implicit Arguments.
 Set Contextual Implicit.
 Set Maximal Implicit Insertion.
 Generalizable All Variables.
 
-Lemma sumbool_map `(f : A -> A') `(g : B -> B') :
-  {A} + {B} -> {A'} + {B'}.
-  firstorder.
-Qed.
+Class Lub (a : Type) :=
+  lub : a -> a -> option a.
 
-Lemma nat_dec (m n : nat) : {m = n} + {m <> n}.
-Proof.
-  intros.
-  eapply sumbool_map.
-  3: apply (eq_nat_decide m n).
-  all: firstorder with arith.
-Qed.
-Arguments nat_dec m n : clear implicits.
+Global Instance Lub_bool : Lub bool :=
+  { lub := fun x y => match x, y with
+                   | true, true => Some true
+                   | false, false => Some false
+                   | _, _ => None
+                   end
+  }.
+
+Inductive T (a : Type) : Type :=
+| thunk (x : a)
+| undefined.
+
+Global Instance Functor_T : Functor T :=
+  { fmap := fun _ _ f x => match x with
+                        | thunk x => thunk (f x)
+                        | undefined => undefined
+                        end
+  }.
+
+Global Instance Monad_T : Monad T :=
+  { ret := @thunk
+  ; bind := fun _ _ c1 c2 => match c1 with
+                          | thunk x => c2 x
+                          | undefined => undefined
+                          end
+  }.
+
+Global Instance Lub_T (a : Type) `{Lub a} : Lub (T a) :=
+  { lub := fun x y => match x, y with
+                   | undefined, _ => Some y
+                   | _, undefined => Some x
+                   | thunk x, thunk y => option_map thunk (lub x y)
+                   end
+  }.
 
 Inductive listA (a : Type) : Type :=
 | nilA : listA a
-| consA : option a -> option (listA a) -> listA a.
+| consA : T a -> T (listA a) -> listA a.
 
-Fixpoint fold_rightA `(f : option a -> option b -> b) (e : b) (xsA : listA a) : b :=
+Fixpoint fold_rightA (a b : Type) (f : T a -> T b -> b) (e : b) (xsA : listA a) : b :=
   match xsA with
   | nilA => e
-  | consA xT xsT => f xT (option_map (fold_rightA f e) xsT)
+  | consA xT xsT => f xT (fmap (fold_rightA f e) xsT)
   end.
+
+Inductive these (a b : Type) : Type :=
+| This (x : a)
+| That (y : b)
+| These (x : a) (y : b).
+
+Global Instance Lub_listA (a : Type) `{Lub a} : Lub (listA a) :=
+  { lub := fix lub_listA xs₁ xs₂ := match xs₁, xs₂ with
+                                    | nilA, nilA => Some nilA
+                                    | consA x₁ xs₁, consA x₂ xs₂ =>
+                                        x <- lub x₁ x₂ ;;
+                                        xs <- @lub _ (@Lub_T _ lub_listA) xs₁ xs₂ ;;
+                                        ret (consA x xs)
+                                    | _, _ => None
+                                    end
+  }.
 
 Axiom TODO : forall a, a.
