Explicit.v
@@ -1,3 +1,9 @@
+Require Import Stdlib.Unicode.Utf8.
+Require Import Stdlib.Lists.List.
+Require Import ExtLib.Structures.Monad.
+Require Import ExtLib.Data.Monads.OptionMonad.
+Require Import ExtLib.Data.Monads.WriterMonad.
+
 Require Import LogicalLaziness.Core.
 Require LogicalLaziness.Lazy.
 
@@ -8,34 +14,209 @@ Generalizable All Variables.
 
 Inductive type : Type :=
 | bool__t : type
-| list__t (a : type) : type
-| t__t (a : type) : type.
+| T__t (alpha : type) : type
+| list__t (alpha : type) : type.
+
+Reserved Notation "⟦ alpha ⟧__eval".
+Fixpoint value (alpha : type) : Type :=
+  match alpha with
+  | bool__t => bool
+  | prod__t alpha beta => ⟦ alpha ⟧__eval * ⟦ beta ⟧__eval
+  | T__t alpha => ⟦ alpha ⟧__eval
+  | list__t alpha => list ⟦ alpha ⟧__eval
+  end
+where "⟦ α ⟧__eval" := (value α).
+
+Reserved Notation "⟦ alpha ⟧__approx".
+Fixpoint approx (α : type) : Type :=
+  match α with
+  | bool__t => bool
+  | prod__t alpha beta => T ⟦ alpha ⟧__approx * T ⟦ beta ⟧__approx
+  | T__t alpha => T ⟦ alpha ⟧__approx
+  | list__t alpha => listA ⟦ alpha ⟧__approx
+  end
+where "⟦ alpha ⟧__approx" := (approx alpha).
 
 Definition Rep : Type :=
   type -> Type.
 
+Definition Hom : Type :=
+  type -> type -> Type.
+
 Section term.
 
+  (* Context (hom : Hom). *)
   Context (rep : Rep).
 
   Inductive term : type -> Type :=
-  | false__t : term bool__t
+  | var__t `(x : rep alpha) : term alpha
+  | let__t (alpha beta : type) (t__1 : term alpha) (t__2 : rep alpha -> term beta) : term beta
   | true__t : term bool__t
-  | if__t (b : term bool__t) `(t : term a) (f : term a) : term a
-  | nil__t : `(term (list__t a))
-  | cons__t `(x : term (t__t a)) (xs : term (t__t (list__t a))) : term (list__t a)
-  | fold_right__t `(f : rep (t__t a) -> rep (t__t b) -> term b) (e : term b) (xs : term (list__t a)) : term b
-  | let__t `(t1 : term a) `(t2 : rep a -> term b) : term b
-  | var__t `(x : rep a) : term a
-  | tick__t `(t : term a) : term a
-  | lazy__t `(t : term a) : term (t__t a)
-  | force__t `(t : term (t__t a)) : term a.
+  | false__t : term bool__t
+  | if__t (b : term bool__t) `(t : term alpha) (f : term alpha) : term alpha
+  | proj1__t (alpha beta : type) : term (prod__t alpha beta) -> term alpha
+  | proj2__t (alpha beta : type) : term (prod__t alpha beta) -> term beta
+  | nil__t : `(term (list__t alpha))
+  | cons__t `(x : term (T__t alpha)) (xs : term (T__t (list__t alpha))) : term (list__t alpha)
+  | fold_right__t `(f : rep (T__t alpha) -> rep (T__t beta) -> term beta) (e : term beta) (xs : term (list__t alpha)) : term beta
+  | tick__t `(t : term alpha) : term alpha
+  | lazy__t `(t : term alpha) : term (T__t alpha)
+  | force__t `(t : term (T__t alpha)) : term alpha.
+
+End term.
+
+(* Fixpoint map__term {rep__1 rep__2 : Rep} (eta : forall alpha, rep__1 alpha -> rep__2 alpha) {alpha : type} (t : term rep__1 alpha) : term rep__2 alpha := *)
+(*   match t with *)
+(*   | var__t x => var__t (eta _ x) *)
+(*   | let__t t__1 k__2 => let__t (map__term eta t__1) (fun x => map__term eta (k__2 x)) *)
+(*   | true__t => true *)
+(*   | false__t => false *)
+(*   | if__t t__1 t__2 t__3 => if__t (map__term eta t__1) (map__term eta t__2) (map__term eta t__3) *)
+(*   | cons__t t__1 t__2 => cons__t (map__term eta t__1) (map__term eta t__2) *)
+(*   | fold_right__t k__1 t__2 t__3 => fold_right__t (fun x__1 x__2 => map__term eta (k__1 x__1 x__2)) (map__term eta t__2) (map__term eta t__3) *)
+(*   | tick__t t__1 => tick__t (map__term eta t__1) *)
+(*   | lazy__t t__1 => lazy__t (map__term eta t__1) *)
+(*   | force__t t__1 => force__t (map__term eta t__1) *)
+(*   end. *)
+
+
+(* Reserved Notation "⟦ t ⟧__eval". *)
+(* Fixpoint eval (alpha : type) (t : term value alpha) : ⟦alpha⟧__eval := *)
+(*   match t with *)
+(*   | var__t x => x *)
+(*   | let__t t₁ k₂ => eval (k₂ ⟦t₁⟧__eval) *)
+(*   | true__t => true *)
+(*   | false__t => false *)
+(*   | if__t t₁ t₂ t₃ => if ⟦t₁⟧__eval then ⟦t₂⟧__eval else ⟦t₃⟧__eval *)
+(*   | nil__t => nil *)
+(*   | cons__t t₁ t₂ => cons ⟦t₁⟧__eval ⟦t₂⟧__eval *)
+(*   | fold_right__t k₁ t₂ t₃ => fold_right (fun x₁ x₂ => ⟦k₁ x₁ x₂⟧__eval) ⟦t₂⟧__eval ⟦t₃⟧__eval *)
+(*   | tick__t t₁ => ⟦t₁⟧__eval *)
+(*   | force__t t₁ => ⟦t₁⟧__eval *)
+(*   | lazy__t t₁ => ⟦t₁⟧__eval *)
+(*   end *)
+(* where "⟦ t ⟧__eval" := (eval t). *)
+
+(* Fixpoint hom__demand : Hom := *)
+(*   (* fun alpha beta => ⟦alpha⟧__eval -> ⟦beta⟧__eval * ⟦alpha⟧__approx. *) *)
+(*   fun alpha beta => ⟦alpha⟧__eval -> term hom__demand value beta. *)
+
+Fixpoint demand (alpha : type) (t : term value α) : approx α → nat :=
+  (* let demand1 (α : type) (t : term value α) *)
+  match t with
+  | var__t _ => fun _ => 0
+  | let__t t₁ k₂ => fun d => let c__1 := demand (k₂ ⟦t₁⟧__eval) d in
+                         let c₂ := demand t₁ d
+  | _ => TODO
+  end.
+
+Inductive lt : ∀ α, approx α -> approx α -> Prop :=
+| lt_refl {α} (x : ⟦ α ⟧ₐ) : lt _ x x
+| lt_undefined {α} (x : ⟦ T__t α ⟧ₐ) :
+  lt (T__t α) undefined x
+| lt_t {α} (x y : ⟦ α ⟧ₐ) :
+  lt α x y ->
+  lt (T__t α) (thunk x) (thunk y)
+| lt_cons {α} (x₁ x₂ : ⟦ T__t α ⟧ₐ) (xs₁ xs₂ : ⟦ T__t (listA__t α) ⟧ₐ) :
+  lt (T__t α) x₁ x₂ →
+  lt (T__t (listA__t α)) xs₁ xs₂ →
+  lt (listA__t α) (consA x₁ xs₁) (consA x₂ xs₂).
+
+(* Import MonadNotation. *)
+(* Open Scope monad_scope. *)
+
+Fixpoint lub' {α : type} : ⟦ α ⟧ₐ → ⟦ α ⟧ₐ → option ⟦ α ⟧ₐ :=
+  match α with
+  | bool__t => Lub_bool
+  | T__t _ => @Lub_T _ lub'
+  | listA__t _ => @Lub_listA _ lub'
+  end.
+
+(*   match α return ⟦ α ⟧ₐ → ⟦ α ⟧ₐ → option ⟦ α ⟧ₐ with *)
+(*   | bool__t => fun v₁ v₂ => match v₁, v₂ with *)
+(*                         | true, true => Some true *)
+(*                         | false, false => Some false *)
+(*                         | _, _ => None *)
+(*                         end *)
+(*   | T__t α => fun v₁ v₂ => match v₁, v₂ with *)
+(*                        | undefined, _ => Some v₂ *)
+(*                        | _, undefined => Some v₁ *)
+(*                        | thunk v₁₁, thunk v₁₂ => option_map thunk (lub v₁₁ v₁₂) *)
+(*                        end *)
+(*   | listA__t α => *)
+(*       fun v₁ v₂ =>  *)
+
+      (* fun v₁ v₂ => match v₁, v₂ with *)
+      (*                      | nilA, nilA => Some nilA *)
+      (*                      | consA v₁₁ v₁₂, consA v₂₁ v₂₂ => *)
+      (*                          v₁' <- match v₁₁, v₂₁ with *)
+      (*                                | undefined, _ => Some v₂₁ *)
+      (*                                | _, undefined => Some v₁₁ *)
+      (*                                | thunk v₁₁₁, thunk v₂₁₁ => option_map thunk (lub v₁₁₁ v₂₁₁) *)
+      (*                                end ;; *)
+      (*                          v₂' <- match v₁₂, v₂₂ with *)
+      (*                                | undefined, _ => Some v₂₂ *)
+      (*                                | _, undefined => Some v₁₂ *)
+      (*                                | thunk v₁₂₁, thunk v₂₂₁ => option_map thunk (lub (v₁₂₁ : ⟦ listA__t _ ⟧ₐ) v₂₂₁) *)
+      (*                                end ;; *)
+      (*                          TODO *)
+      (*                      | _, _ => None *)
+      (*                      end *)
+  end.
+
+  intros v₁ v₂.
+  destruct α.
+  - exact TODO.
+  - destruct v₁.
+    + destruct v₂.
+      * exact (option_map thunk (lub _ x x0)).
+      * exact None.
+    + exact (Some v₂).
+  - destruct v₁, v₂.
+    + exact (Some nilA).
+    + exact None.
+    + exact None.
+    + destruct t, t1.
+      * admit.
+         
+  
+  
+  match α as α return ⟦ α ⟧ₐ → ⟦ α ⟧ₐ → option ⟦ α ⟧ₐ with
+  | listA__t α =>
+      fun v₁ v₂ => match v₁, v₂ with
+                (* | nilA, nilA => Some nilA *)
+                | consA v₁₁ v₁₂, consA v₂₁ v₂₂ =>
+                    v₁' <- match v₁₁, v₂₁ with
+                          | None, _ => Some v₂₁
+                          | Some x, Some y => Some (lub x y)
+                          | _, _ => None
+                          end ;;
+                    v₂' <- match v₁₂, v₂₂ with
+                          | None, _ => Some v₂₂
+                          | Some x, Some y => Some (lub (x : ⟦ listA__t _ ⟧ₐ) y)
+                          | _, _ => None
+                          end ;;
+                    ret (consA v₁' v₂')
+                    (* match lub' v₁₁ v₂₁ lub, lub' (v₁₂ : ⟦ t__t (listA__t α) ⟧ₐ) v₂₂ lub with *)
+                    (* | Some v₁', Some v₂' => Some (consA v₁' v₂') *)
+                    (* | _, _ => None *)
+                    (* end *)
+                      (* | _, _ => None *)
+                | _, _ => TODO
+                end
+  | _ => TODO
+  end.
+  
+Section translate.
 
   Fixpoint translate_type (a : Lazy.type) : type :=
     match a with
     | Lazy.bool__t => bool__t
     | Lazy.list__t a => list__t (translate_type a)
     end.
+
+  Context (rep : Rep).
+  Local Notation term := (term rep).
 
   Definition rep' : Lazy.Rep :=
     fun a => rep (t__t (translate_type a)).
@@ -67,4 +248,4 @@ Section term.
                    (fun x => translate_term (k x)))
     end.
 
-End term.
+End translate.
