Lazy.v
@@ -19,77 +19,16 @@ Section term.
   Context (rep : Rep).
 
   Inductive term : type -> Type :=
-  | false__t : term bool__t
   | true__t : term bool__t
-  | if__t `(c : rep bool__t) `(t : term α) (f : term α) : term α
+  | false__t : term bool__t
+  | if__t `(c : term bool__t) `(t : term α) (f : term α) : term α
   | nil__t : `(term (list__t α))
-  | cons__t `(x : rep α) (xs : rep (list__t α)) : term (list__t α)
-  | fold_right__t `(f : rep α -> rep β -> term β) (e : rep β) (xs : rep (list__t α)) : term β
+  | cons__t `(x : term α) (xs : term (list__t α)) : term (list__t α)
+  | fold_right__t `(f : rep α -> rep β -> term β) (e : term β) (xs : term (list__t α)) : term β
   | var__t `(r : rep α) : term α
   | let__t {α β} (d : term α) (t : rep α -> term β) : term β.
 
 End term.
 
 Definition program (a : type) : Type :=
-  forall rep, term rep a.
-
-Fixpoint value (α : type) : Type :=
-  match α with
-  | bool__t => bool
-  | list__t α => list (value α)
-  end.
-
-Inductive whnf (rep : Rep) : type → Type :=
-| true__v : whnf rep bool__t
-| false__v : whnf rep bool__t
-| nil__v : `(whnf rep (list__t α))
-| cons__v `(x : term rep α) (xs : term rep (list__t α)) : whnf rep (list__t α).
-
-Module Type Heap.
-  Axiom ix : Type.
-  Axiom t : Type : ix -> type.
-  Axiom ix : Type.
-  Axiom key : type → Type.
-  Axiom extend : `(term key α → t -> key α * t).
-  Axiom lookup : `(key α → t → option (term key α)).
-
-  Axiom In : 
-End Heap.
-
-Module eval (H : Heap).
-  Fixpoint eval (Γ : H.t) `(t : term key α) : option (whnf key α * H.t * nat).
-    refine (match t with
-            | false__t => Some (false__v, Γ, 1)
-            | true__t => Some (true__v, Γ, 1)
-            | if__t c t f => match eval Γ _ _ (var__t c) with
-                            | Some (c, Δ, m) =>
-                                let k := match c with
-                                         | true__v => t
-                                         | false__v => f
-                                         | _ => _
-                                         end in
-                                let (r, Θ, n) := eval Γ _ _ k
-                                               in Some (r, Θ, m + n)
-                            | None => None
-                            end
-            | _ => TODO
-            end).
-
-Section env.
-
-  Context (rep : Rep).
-
-  Definition env :=
-    forall {α : type}, rep α → option (value α).
-
-  (* Axiom extend : forall (e : env) `(r : rep α) (v : value α), env. *)
-
-  Context (rep_term : forall {α}, term rep α → rep α).
-
-  Fixpoint denote_term `(e : env) `(t : term rep α) : value α * nat :=
-    match t in term _ α return value α * nat with
-    | false__t => (false, 1)
-    | true__t => (true, 1)
-    | let__t d b => denote_term e (b (rep_term d))
-    | _ => TODO
-    end.
+  forall {rep}, term rep a.
